src/program_proof/simplepb/pb_ghost.v
@@ -266,6 +266,15 @@ Proof.
   done.
 Qed.
 
+Lemma ghost_get_proposal_facts γsys γsrv epoch σ sealed :
+  own_replica_ghost γsys γsrv epoch σ sealed -∗
+  is_proposal_lb γsys epoch σ ∗
+  is_proposal_facts γsys epoch σ.
+Proof.
+  iNamed 1.
+  iFrame "#".
+Qed.
+
 Lemma ghost_accept γsys γsrv epoch epoch' σ σ' :
   int.nat epoch ≤ int.nat epoch' →
   length σ ≤ length σ' →
